Added termination condition to Z-Machines

Z_Machine.thy
@@ -3,7 +3,7 @@ theory Z_Machine
     "HOL-Library.Code_Target_Numeral" "ITree_Simulation.Code_Rational"
     "Explorer.Explorer" Show_Record
   keywords "zmachine" "zoperation" :: "thy_decl_block"
-    and "over" "init" "invariant" "operations" "params" "pre" "update" "\<in>" "promote" "emit"
+    and "over" "init" "invariant" "operations" "until" "params" "pre" "update" "\<in>" "promote" "emit"
 begin
 
 named_theorems z_machine_defs
@@ -56,8 +56,8 @@ lemma wlp_Vis: "wlp (\<lambda> s. Vis (F s)) P = (\<forall> e\<in>dom F. wlp (\<
 definition z_machine_main :: "(('e::show, 's) htree) list \<Rightarrow> ('e, 's) htree" where
 "z_machine_main Ops = (foldr (\<box>) Ops Stop)"
 
-definition z_machine :: "('s::default) subst \<Rightarrow> ('s \<Rightarrow> bool) \<Rightarrow> (('e::show, 's) htree) list \<Rightarrow> 'e process" where
-[code_unfold]: "z_machine Init Inv Ops = process Init (loop (z_machine_main Ops))"
+definition z_machine :: "('s::default) subst \<Rightarrow> ('s \<Rightarrow> bool) \<Rightarrow> (('e::show, 's) htree) list \<Rightarrow> ('s \<Rightarrow> bool) \<Rightarrow> 'e process" where
+[code_unfold]: "z_machine Init Inv Ops End = process Init (iterate (Not \<circ> End) (z_machine_main Ops))"
 
 (*
 definition z_machine :: "('s::default) subst \<Rightarrow> ('e, 's) htree list \<Rightarrow> 'e process" where
@@ -69,9 +69,9 @@ lemma deadlock_free_z_machine:
   assumes 
     "Init establishes Inv"
     "\<And> E. E\<in>set Events \<Longrightarrow> E preserves Inv"
-    "`Inv \<longrightarrow> dfp (foldr (\<box>) Events Stop)`"
-  shows "deadlock_free (z_machine Init Inv Events)"
-proof (simp add: z_machine_def z_machine_main_def, rule deadlock_free_processI, rule deadlock_free_init_loop[where P="Inv"], rule assms(1), simp_all)
+    "`\<not> End \<and> Inv \<longrightarrow> dfp (foldr (\<box>) Events Stop)`"
+  shows "deadlock_free (z_machine Init Inv Events End)"
+proof (simp add: z_machine_def z_machine_main_def, rule deadlock_free_processI, rule deadlock_free_init_iterate[where P="Inv"], rule assms(1), simp_all)
   from assms(2) show "\<^bold>{Inv\<^bold>} foldr (\<box>) Events Stop \<^bold>{Inv\<^bold>}"
   proof (induct Events)
     case Nil
@@ -81,7 +81,7 @@ proof (simp add: z_machine_def z_machine_main_def, rule deadlock_free_processI, 
     then show ?case
       by (metis foldr.simps(2) hl_choice list.set_intros(1) list.set_intros(2) o_apply)
   qed
-  show "`Inv \<longrightarrow> dfp (foldr (\<box>) Events Stop)`"
+  show "`\<not> End \<and> Inv \<longrightarrow> dfp (foldr (\<box>) Events Stop)`"
     using assms(3) by auto
 qed
 
